AlgoLib.lean
@@ -110,3 +110,6 @@ import AlgoLib.Experimental.RAM.Tests.ContractFrontend
 import AlgoLib.Experimental.RAM.Tests.MixedFrontend
 import AlgoLib.Experimental.RAM.Prototype.Composition.SortingExecution
 import AlgoLib.Experimental.RAM.Tests.MixedAxioms
+
+import AlgoLib.Experimental.RAM.Tests.PaperLoops
+import AlgoLib.Experimental.RAM.Tests.PaperLoopAxioms
